Change naming to snake case with new names instead of camel case

new/proof/github_com/goose_lang/goose/model/channel/idiom/done/done.v
@@ -52,10 +52,10 @@ Definition Notified (γ : done_names) (Q : iProp Σ) : iProp Σ :=
     saved_prop_own prop_gname (DfracOwn (1/2)) Q.
 
 Definition is_done (γ : done_names) (ch : loc) : iProp Σ :=
-  IsChan ch γ.(chan_name) ∗
+  is_chan ch γ.(chan_name) ∗
   inv nroot (
     ∃ (s : chan_rep.t V) (m : gmap nat gname) (Qs: list (iProp Σ)),
-      "Hch" ∷ OwnChan ch s γ.(chan_name) ∗
+      "Hch" ∷ own_chan ch s γ.(chan_name) ∗
       "Hmap" ∷ ghost_map_auth γ.(receivers_map_name) (1/2)%Qp m ∗
       match s with
       | chan_rep.Idle => True
@@ -188,8 +188,8 @@ iMod (saved_prop_update (R ∗ Q) with "Hsp") as "Hsp".
 Qed.
 
 Lemma start_done (ch : loc) (γ : chan_names) :
-  IsChan ch γ -∗
-  OwnChan ch chan_rep.Idle γ ={⊤}=∗
+  is_chan ch γ -∗
+  own_chan ch chan_rep.Idle γ ={⊤}=∗
   ∃ γdone, is_done γdone ch ∗ Notify γdone True.
 Proof.
   iIntros "#Hch Hoc".
@@ -206,7 +206,7 @@ Proof.
   |}).
   iMod (inv_alloc nroot _ (
     ∃ s m Qs,
-      "Hch" ∷ OwnChan ch s γ ∗
+      "Hch" ∷ own_chan ch s γ ∗
       "Hmap" ∷ ghost_map_auth γmap (1/2)%Qp m ∗
       match s with
       | chan_rep.Idle => True
@@ -246,8 +246,8 @@ Proof.
   }
 Qed.
 
-Lemma done_IsChan γ ch :
-  is_done γ ch ⊢ IsChan ch γ.(chan_name).
+Lemma done_is_chan γ ch :
+  is_done γ ch ⊢ is_chan ch γ.(chan_name).
 Proof.
   iDestruct 1 as "[$ _]".
 Qed.
@@ -327,7 +327,7 @@ Lemma done_receive_au γ ch Q  :
   Notified γ Q -∗
   ▷ (Q -∗ Φ (default_val V) false) -∗
   £1 ∗ £1 ∗ £1 ∗ £1 -∗
-  RecvAU ch γ.(chan_name) (λ (v:V) (ok:bool), Φ v ok).
+  recv_au ch γ.(chan_name) (λ (v:V) (ok:bool), Φ v ok).
 Proof.
   intros Φ.
   iIntros "#Hdone".
@@ -355,7 +355,7 @@ Proof.
       iNext. iFrame. iExists []. done.
     }
     iModIntro.
-    unfold RecvNestedAU.
+    unfold recv_nested_au.
     iInv "Hinv" as "Hinv_open1" "Hinv_close".
     iMod (lc_fupd_elim_later with "[$] Hinv_open1") as "Hinv_open1".
     iNamed "Hinv_open1".
